examples/modular_inversion/proofs/gcd_props.ec
@@ -11,3 +11,9 @@ lemma gcd3 u v : gcd u v = gcd (u - v) v. smt. qed.
 lemma gcd4 u v : gcd u v = gcd v u. smt. qed.
 lemma gcd5 u v : gcd u v = gcd (-u) v. smt. qed.
 lemma gcd6 t v : gcd t v = gcd (t - v) v. smt. qed.
+
+
+
+op inv : int -> int -> int.
+  (* add proper conditions *)
+axiom inv_ax u v : (inv u v) * v %% u = 1. 
